src/Spec/Example.v
@@ -1,0 +1,121 @@
+Require Import Helpers.Helpers.
+Require Import Helpers.ListStuff.
+Require Import ConcurProc.
+
+Global Set Implicit Arguments.
+Global Generalizable All Variables.
+
+
+(** Opcodes *)
+
+Inductive opT : Type -> Type :=
+| Inc : opT nat
+| Noop : opT unit.
+
+Inductive opHiT : Type -> Type :=
+| IncTwice : opHiT nat
+| Noop2 : opHiT unit.
+
+Inductive opHi2T : Type -> Type :=
+.
+
+
+(** State *)
+
+Definition State := forall (tid : nat), nat.
+
+Definition init_state : State := fun tid' => 4.
+
+Definition state_upd (s : State) (tid : nat) (val : nat) :=
+  fun tid' =>
+    if tid' == tid then val else s tid'.
+
+Definition inc s tid :=
+  state_upd s tid (s tid + 1).
+
+Definition inc2 s tid :=
+  state_upd s tid (s tid + 2).
+
+
+(** Semantics *)
+
+Inductive op_step : forall T, opT T -> nat -> State -> T -> State -> Prop :=
+| StepInc : forall tid s,
+  op_step Inc tid s (s tid + 1) (inc s tid)
+| StepNoop : forall tid s,
+  op_step Noop tid s tt s.
+
+Inductive opHi_step : forall T, opHiT T -> nat -> State -> T -> State -> Prop :=
+| StepIncTwice : forall tid s,
+  opHi_step IncTwice tid s (s tid + 2) (inc2 s tid)
+| StepNoop2 : forall tid s,
+  opHi_step Noop2 tid s tt s.
+
+
+(** Implementations *)
+
+Definition inc_twice_impl :=
+  _ <- OpCallHi IncTwice;
+  _ <- Op Inc;
+  i2 <- Op Inc;
+  OpRetHi i2.
+
+Definition p1 :=
+  _ <- inc_twice_impl;
+  Ret tt.
+
+Definition ts := threads_empty [[ 1 := Proc p1 ]].
+
+
+Definition p2 : proc opHiT opHi2T _ :=
+  _ <- Op IncTwice;
+  Ret tt.
+
+Definition ts2 := threads_empty [[ 1 := Proc p2 ]].
+
+
+
+(** Example traces *)
+
+Ltac exec_one tid' :=
+  eapply ExecOne with (tid := tid');
+    [ rewrite thread_upd_eq; reflexivity | | autorewrite with t ].
+
+Hint Constructors op_step.
+Hint Constructors opHi_step.
+
+Definition ex_trace :
+  { t : trace opT opHiT | exec op_step init_state ts t }.
+Proof.
+  eexists.
+  unfold ts.
+  unfold init_state.
+  exec_one 1; eauto; simpl; autorewrite with t.
+  exec_one 1; eauto; simpl; autorewrite with t.
+  exec_one 1; eauto; simpl; autorewrite with t.
+  exec_one 1; eauto; simpl; autorewrite with t.
+  exec_one 1; eauto; simpl; autorewrite with t.
+  exec_one 1; eauto; simpl; autorewrite with t.
+  exec_one 1; eauto; simpl; autorewrite with t.
+  exec_one 1; eauto; simpl; autorewrite with t.
+  exec_one 1; eauto; simpl; autorewrite with t.
+  eapply ExecEmpty; eauto.
+Defined.
+
+Eval compute in (proj1_sig ex_trace).
+
+
+Definition ex_trace2 :
+  { t : trace opHiT opHi2T | exec opHi_step init_state ts2 t }.
+Proof.
+  eexists.
+  unfold ts2.
+  unfold init_state.
+  exec_one 1; eauto; simpl; autorewrite with t.
+  exec_one 1; eauto; simpl; autorewrite with t.
+  exec_one 1; eauto; simpl; autorewrite with t.
+  exec_one 1; eauto; simpl; autorewrite with t.
+  eapply ExecEmpty; eauto.
+Defined.
+
+Eval compute in (proj1_sig ex_trace2).
